lean/Nucleus/Nucleus/Json.lean
@@ -1,4 +1,5 @@
 import Nucleus.Json.Raw
+import Nucleus.Json.Containers
 import Nucleus.Json.Extensional
 import Nucleus.Json.Ordered
 import Nucleus.Json.Validate
